Update Polymorph and add Makefile

src/StructuredEncryption/runtimes/net/Generated/CryptoAction.cs
@@ -1,0 +1,19 @@
+// Copyright Amazon.com Inc. or its affiliates. All Rights Reserved.
+// SPDX-License-Identifier: Apache-2.0
+// Do not modify this file. This file is machine generated, and any changes to it will be overwritten.
+using System;
+ using AWS.Cryptography.StructuredEncryption; namespace AWS.Cryptography.StructuredEncryption {
+ using Amazon.Runtime; public class CryptoAction : ConstantClass {
+
+ 
+ public static readonly CryptoAction ENCRYPT_AND_SIGN = new CryptoAction ("ENCRYPT_AND_SIGN");
+ 
+ public static readonly CryptoAction SIGN_ONLY = new CryptoAction ("SIGN_ONLY");
+ 
+ public static readonly CryptoAction IGNORE = new CryptoAction ("IGNORE");
+ public static readonly  CryptoAction [] Values =  {
+ ENCRYPT_AND_SIGN , IGNORE , SIGN_ONLY
+} ;
+ public CryptoAction (string value) : base(value) {}
+}
+}
