src/StructuredEncryption/runtimes/net/Generated/CryptoSchema.cs
@@ -1,0 +1,28 @@
+// Copyright Amazon.com Inc. or its affiliates. All Rights Reserved.
+// SPDX-License-Identifier: Apache-2.0
+// Do not modify this file. This file is machine generated, and any changes to it will be overwritten.
+using System;
+ using AWS.Cryptography.StructuredEncryption; namespace AWS.Cryptography.StructuredEncryption {
+ public class CryptoSchema {
+ private AWS.Cryptography.StructuredEncryption.CryptoSchemaContent _content ;
+ private System.Collections.Generic.Dictionary<string, AWS.Cryptography.StructuredEncryption.CryptoAction> _attributes ;
+ public AWS.Cryptography.StructuredEncryption.CryptoSchemaContent Content {
+ get { return this._content; }
+ set { this._content = value; }
+}
+ internal bool IsSetContent () {
+ return this._content != null;
+}
+ public System.Collections.Generic.Dictionary<string, AWS.Cryptography.StructuredEncryption.CryptoAction> Attributes {
+ get { return this._attributes; }
+ set { this._attributes = value; }
+}
+ internal bool IsSetAttributes () {
+ return this._attributes != null;
+}
+ public void Validate() {
+ if (!IsSetContent()) throw new System.ArgumentException("Missing value for required property 'Content'");
+
+}
+}
+}
