src/StructuredEncryption/runtimes/net/Generated/DecryptStructureInput.cs
@@ -1,0 +1,29 @@
+// Copyright Amazon.com Inc. or its affiliates. All Rights Reserved.
+// SPDX-License-Identifier: Apache-2.0
+// Do not modify this file. This file is machine generated, and any changes to it will be overwritten.
+using System;
+ using AWS.Cryptography.StructuredEncryption; namespace AWS.Cryptography.StructuredEncryption {
+ public class DecryptStructureInput {
+ private AWS.Cryptography.StructuredEncryption.StructuredData _ciphertextStructure ;
+ private AWS.Cryptography.StructuredEncryption.CryptoSchema _cryptoSchema ;
+ public AWS.Cryptography.StructuredEncryption.StructuredData CiphertextStructure {
+ get { return this._ciphertextStructure; }
+ set { this._ciphertextStructure = value; }
+}
+ internal bool IsSetCiphertextStructure () {
+ return this._ciphertextStructure != null;
+}
+ public AWS.Cryptography.StructuredEncryption.CryptoSchema CryptoSchema {
+ get { return this._cryptoSchema; }
+ set { this._cryptoSchema = value; }
+}
+ internal bool IsSetCryptoSchema () {
+ return this._cryptoSchema != null;
+}
+ public void Validate() {
+ if (!IsSetCiphertextStructure()) throw new System.ArgumentException("Missing value for required property 'CiphertextStructure'");
+ if (!IsSetCryptoSchema()) throw new System.ArgumentException("Missing value for required property 'CryptoSchema'");
+
+}
+}
+}
