Makefile
@@ -1,0 +1,15 @@
+build:
+	cd src/StructuredEncryption/src;\
+	dotnet build
+
+test: build
+	cd src/StructuredEncryption/runtimes/net;\
+	dotnet test -f netcoreapp3.1 Test
+
+generate-models:
+	cd polymorph/smithy-dotnet;\
+	./gradlew run --args="\
+		-m src/StructuredEncryption/model\
+		-namespace aws.cryptography.structuredEncryption\
+		--output-dotnet src/StructuredEncryption/runtimes/net/Generated\
+		-d src/StructuredEncryption/model"
